proofs/prelude/math.bpl
@@ -1,120 +1,115 @@
 // ----------------------------------------
 // Mathematical sets, sequences, etc.
-// 
+//
+// These axioms are adapted from Dafny's axioms,
+// instantiated to type Invoc because CIVL does not support polymorphic Boogie:
+// https://github.com/boogie-org/boogie/issues/122
+//
+// The dafny axioms were taken from
+// https://github.com/Microsoft/dafny/blob/master/Binaries/DafnyPrelude.bpl
+// which had the following notice at the top of the file:
+// Dafny prelude
+// Created 9 February 2008 by Rustan Leino.
+// Converted to Boogie 2 on 28 June 2008.
+// Edited sequence axioms 20 October 2009 by Alex Summers.
+// Modified 2014 by Dan Rosen.
+// Copyright (c) 2008-2014, Microsoft.
 // ----------------------------------------
 
 
-// ---------- Types and axiomatization of sets
+// ---------- Types and axiomatization of sets (of invocations)
 
-// Sets of invocations
-type SetInvoc;
+type SetInvoc = [Invoc]bool;
 
-const Set_empty: SetInvoc;
+function Set_card(SetInvoc): int;
+axiom (forall s: SetInvoc :: { Set_card(s) } 0 <= Set_card(s));
 
-function Set(n: Invoc) : SetInvoc;  // singleton set
+function Set_empty(): SetInvoc;
+axiom (forall o: Invoc :: { Set_empty()[o] } !Set_empty()[o]);
+axiom (forall s: SetInvoc :: { Set_card(s) }
+  (Set_card(s) == 0 <==> s == Set_empty()) &&
+  (Set_card(s) != 0 ==> (exists x: Invoc :: s[x])));
 
-function Set_elem(n: Invoc, s: SetInvoc) : bool;
+// the empty set could be of anything
+//axiom (forall t: Ty :: { $Is(Set_empty() : [Invoc]bool, TSet(t)) } $Is(Set_empty() : [Invoc]bool, TSet(t)));
 
-function Set_subset(s: SetInvoc, t: SetInvoc) : bool;
+function Set(Invoc): SetInvoc;
+axiom (forall r: Invoc :: { Set(r) } Set(r)[r]);
+axiom (forall r: Invoc, o: Invoc :: { Set(r)[o] } Set(r)[o] <==> r == o);
+axiom (forall r: Invoc :: { Set_card(Set(r)) } Set_card(Set(r)) == 1);
 
-function Set_equal(s, t: SetInvoc) : bool;  // helper function to prove sets are equal
+function Set_add(SetInvoc, Invoc): SetInvoc;
+axiom (forall a: SetInvoc, x: Invoc, o: Invoc :: { Set_add(a,x)[o] }
+  Set_add(a,x)[o] <==> o == x || a[o]);
+axiom (forall a: SetInvoc, x: Invoc :: { Set_add(a, x) }
+  Set_add(a, x)[x]);
+axiom (forall a: SetInvoc, x: Invoc, y: Invoc :: { Set_add(a, x), a[y] }
+  a[y] ==> Set_add(a, x)[y]);
+axiom (forall a: SetInvoc, x: Invoc :: { Set_card(Set_add(a, x)) }
+  a[x] ==> Set_card(Set_add(a, x)) == Set_card(a));
+axiom (forall a: SetInvoc, x: Invoc :: { Set_card(Set_add(a, x)) }
+  !a[x] ==> Set_card(Set_add(a, x)) == Set_card(a) + 1);
 
-// extensionality
-axiom (forall s, t: SetInvoc :: {Set_equal(s, t)}
-  (forall n: Invoc :: Set_elem(n, s) <==> Set_elem(n, t)) ==> Set_equal(s, t) && s == t);
+function Set_union(SetInvoc, SetInvoc): SetInvoc;
+axiom (forall a: SetInvoc, b: SetInvoc, o: Invoc :: { Set_union(a,b)[o] }
+  Set_union(a,b)[o] <==> a[o] || b[o]);
+axiom (forall a, b: SetInvoc, y: Invoc :: { Set_union(a, b), a[y] }
+  a[y] ==> Set_union(a, b)[y]);
+axiom (forall a, b: SetInvoc, y: Invoc :: { Set_union(a, b), b[y] }
+  b[y] ==> Set_union(a, b)[y]);
+axiom (forall a, b: SetInvoc :: { Set_union(a, b) }
+  Set_disjoint(a, b) ==>
+    Set_diff(Set_union(a, b), a) == b &&
+    Set_diff(Set_union(a, b), b) == a);
+// Follows from the general union axiom, but might be still worth including, because disjoint union is a common case:
+// axiom (forall a, b: SetInvoc :: { Set_card(Set_union(a, b)) }
+//   Set_disjoint(a, b) ==>
+//     Set_card(Set_union(a, b)) == Set_card(a) + Set_card(b));
 
-// Set_empty is a subset of anything
-axiom (forall s: SetInvoc :: Set_subset(Set_empty, s));
+function Set_inter(SetInvoc, SetInvoc): SetInvoc;
+axiom (forall a: SetInvoc, b: SetInvoc, o: Invoc :: { Set_inter(a,b)[o] }
+  Set_inter(a,b)[o] <==> a[o] && b[o]);
 
-// Nothing is an elem of Set_empty
-axiom (forall n: Invoc :: !Set_elem(n, Set_empty));
+axiom (forall a, b: SetInvoc :: { Set_union(Set_union(a, b), b) }
+  Set_union(Set_union(a, b), b) == Set_union(a, b));
+axiom (forall a, b: SetInvoc :: { Set_union(a, Set_union(a, b)) }
+  Set_union(a, Set_union(a, b)) == Set_union(a, b));
+axiom (forall a, b: SetInvoc :: { Set_inter(Set_inter(a, b), b) }
+  Set_inter(Set_inter(a, b), b) == Set_inter(a, b));
+axiom (forall a, b: SetInvoc :: { Set_inter(a, Set_inter(a, b)) }
+  Set_inter(a, Set_inter(a, b)) == Set_inter(a, b));
+axiom (forall a, b: SetInvoc :: { Set_card(Set_union(a, b)) }{ Set_card(Set_inter(a, b)) }
+  Set_card(Set_union(a, b)) + Set_card(Set_inter(a, b)) == Set_card(a) + Set_card(b));
 
-// Set(n) definition
-axiom (forall n1, n2: Invoc :: {Set_elem(n2, Set(n1))}
-  Set_elem(n2, Set(n1)) <==> n2 == n1);
+function Set_diff(SetInvoc, SetInvoc): SetInvoc;
+axiom (forall a: SetInvoc, b: SetInvoc, o: Invoc :: { Set_diff(a,b)[o] }
+  Set_diff(a,b)[o] <==> a[o] && !b[o]);
+axiom (forall a, b: SetInvoc, y: Invoc :: { Set_diff(a, b), b[y] }
+  b[y] ==> !Set_diff(a, b)[y] );
+axiom (forall a, b: SetInvoc ::
+  { Set_card(Set_diff(a, b)) }
+  Set_card(Set_diff(a, b)) + Set_card(Set_diff(b, a))
+  + Set_card(Set_inter(a, b))
+    == Set_card(Set_union(a, b)) &&
+  Set_card(Set_diff(a, b)) == Set_card(a) - Set_card(Set_inter(a, b)));
 
-// subset is reflexive
-axiom (forall s: SetInvoc :: Set_subset(s, s));
+function Set_subset(SetInvoc, SetInvoc): bool;
+axiom(forall a: SetInvoc, b: SetInvoc :: { Set_subset(a,b) }
+  Set_subset(a,b) <==> (forall o: Invoc :: {a[o]} {b[o]} a[o] ==> b[o]));
+// axiom(forall a: SetInvoc, b: SetInvoc ::
+//   { Set_subset(a,b), Set_card(a), Set_card(b) }  // very restrictive trigger
+//   Set_subset(a,b) ==> Set_card(a) <= Set_card(b));
 
-// subset is transitive
-axiom (forall s, t, u: SetInvoc ::
-    {Set_subset(s, t), Set_subset(t, u), Set_subset(s, u)}
-  Set_subset(s, t) && Set_subset(t, u) ==> Set_subset(s, u));
 
-// definition of subset in terms of elem
-axiom (forall s, t: SetInvoc :: {Set_subset(s, t)}
-  (forall n: Invoc :: Set_elem(n, s) ==> Set_elem(n, t)) ==> Set_subset(s, t));
-axiom (forall s, t: SetInvoc, n: Invoc ::
-    {Set_subset(s, t), Set_elem(n, s)} {Set_subset(s, t), Set_elem(n, t)}
-  Set_subset(s, t) && Set_elem(n, s) ==> Set_elem(n, t));
+function Set_equal(SetInvoc, SetInvoc): bool;
+axiom(forall a: SetInvoc, b: SetInvoc :: { Set_equal(a,b) }
+  Set_equal(a,b) <==> (forall o: Invoc :: {a[o]} {b[o]} a[o] <==> b[o]));
+axiom(forall a: SetInvoc, b: SetInvoc :: { Set_equal(a,b) }  // extensionality axiom for sets
+  Set_equal(a,b) ==> a == b);
 
-function Set_union(s1: SetInvoc, s2: SetInvoc) returns (t: SetInvoc);
-
-// union is idempotent
-axiom (forall s: SetInvoc :: s == Set_union(s, s));
-
-// union is associative
-axiom (forall s, t: SetInvoc :: {Set_union(s, t), Set_union(t, s)}
-  Set_union(s, t) == Set_union(t, s));
-
-// union preserves subset
-axiom (forall s1, s2, s3: SetInvoc :: {Set_subset(s1, s2), Set_subset(s1, Set_union(s2, s3))}
-  Set_subset(s1, s2) ==> Set_subset(s1, Set_union(s2, s3)));
-
-// union with empty
-axiom (forall s: SetInvoc :: Set_union(s, Set_empty) == s);
-axiom (forall s: SetInvoc :: Set_union(Set_empty, s) == s);
-
-// union is monotonic w.r.t subset
-// axiom (forall s, t1, t2: SetInvoc ::
-//   Set_subset(t1, t2) ==> Set_subset(Set_union(s, t1), Set_union(s, t2)));
-
-// axiom (forall s, t1, t2: SetInvoc ::
-//   Set_subset(t1, s) && Set_subset(t2, s) ==> Set_subset(Set_union(t1, t2), s));
-
-// relation between union and elem
-axiom (forall n: Invoc, s, t: SetInvoc ::
-    {Set_elem(n, Set_union(s, t)), Set_elem(n, t)}
-    {Set_elem(n, Set_union(s, t)), Set_elem(n, s)}
-  Set_elem(n, Set_union(s, t)) <==> Set_elem(n, s) || Set_elem(n, t));
-
-// intersection
-function Set_inter(s1: SetInvoc, s2: SetInvoc) returns (t: SetInvoc);
-
-// relation between intersection and elem
-axiom (forall n: Invoc, s, t: SetInvoc ::
-    {Set_elem(n, Set_inter(s, t)), Set_elem(n, t)}
-    {Set_elem(n, Set_inter(s, t)), Set_elem(n, s)}
-  Set_elem(n, Set_inter(s, t)) <==> Set_elem(n, s) && Set_elem(n, t));
-
-// intersection with empty
-axiom (forall s: SetInvoc :: Set_inter(s, Set_empty) == Set_empty);
-axiom (forall s: SetInvoc :: Set_inter(Set_empty, s) == Set_empty);
-
-function Set_ofSeq(q: SeqInvoc) returns (s: SetInvoc);
-
-function Set_add(s: SetInvoc, n: Invoc) returns (t: SetInvoc);
-
-// add in terms of union and singleton
-axiom (forall s: SetInvoc, n: Invoc :: {Set_union(s, Set(n))} Set_add(s, n) == Set_union(s, Set(n)));
-
-// Relation between add and elem
-axiom (forall s: SetInvoc, n1, n2: Invoc :: {Set_elem(n1, Set_add(s, n2))}
-  Set_elem(n1, Set_add(s, n2)) <==> n1 == n2 || Set_elem(n1, s));
-axiom (forall s: SetInvoc, n: Invoc :: {Set_elem(n, s), Set_add(s, n)}
-  Set_elem(n, s) ==> Set_add(s, n) == s);
-
-// What happens when you add to empty
-axiom (forall n: Invoc :: {Set_add(Set_empty, n)} Set_add(Set_empty, n) == Set(n));
-
-// Relation between union and elem
-// axiom (forall s, t: SetInvoc, n1: Invoc :: Set_elem(n1, Set_union(s, t))
-//        ==> Set_elem(n1, s) || Set_elem(n1, t));
-
-// add preserves subset relation
-// axiom (forall s, t: SetInvoc, n: Invoc :: Set_subset(s, t) ==> Set_subset(Set_add(s, n), Set_add(t, n)));
-axiom (forall s, t: SetInvoc, n: Invoc :: {Set_subset(s, Set_add(t, n))}
-  Set_subset(s, t) ==> Set_subset(s, Set_add(t, n)));
+function Set_disjoint(SetInvoc, SetInvoc): bool;
+axiom (forall a: SetInvoc, b: SetInvoc :: { Set_disjoint(a,b) }
+  Set_disjoint(a,b) <==> (forall o: Invoc :: {a[o]} {b[o]} !a[o] || !b[o]));
 
 
 // ---------- Types and axiomatization of sequences (of invocations)
@@ -131,14 +126,17 @@ axiom (forall n1, n2: Invoc, s: SeqInvoc :: {Seq_elem(n1, Seq_append(s, n2))}
        Seq_elem(n1, Seq_append(s, n2)) <==> Seq_elem(n1, s) || n1 == n2);
 
 
+// -- New functions and axioms:
+
+function Set_ofSeq(q: SeqInvoc) returns (s: SetInvoc);
+
 // Relation between Set_ofSeq, add, and append
 axiom (forall q: SeqInvoc, n: Invoc :: {Set_ofSeq(Seq_append(q, n))}
   Set_ofSeq(Seq_append(q, n)) == Set_add(Set_ofSeq(q), n));
 
 // Relation between Set_ofSeq, Set_elem, and Seq_elem
-axiom (forall q: SeqInvoc, n: Invoc :: {Set_elem(n, Set_ofSeq(q))}
-  Seq_elem(n, q) <==> Set_elem(n, Set_ofSeq(q)));
-
+axiom (forall q: SeqInvoc, n: Invoc :: {Set_ofSeq(q)[n]}
+  Seq_elem(n, q) <==> Set_ofSeq(q)[n]);
 
 // Distinct sequences
 function Seq_distinct(q: SeqInvoc) : bool;
@@ -160,12 +158,12 @@ axiom (forall q: SeqInvoc, s: SetInvoc, n: Invoc :: {Seq_restr(Seq_append(q, n),
   ==> Seq_restr(Seq_append(q, n), s) == Seq_restr(q, s));
 axiom (forall q: SeqInvoc, s: SetInvoc, n: Invoc ::
     {Seq_restr(Seq_append(q, n), Set_add(s, n))}
-  Seq_distinct(Seq_append(q, n)) && !Set_elem(n, s)
+  Seq_distinct(Seq_append(q, n)) && !s[n]
   ==> Seq_restr(Seq_append(q, n), Set_add(s, n)) == Seq_append(Seq_restr(q, s), n));
 
 // Relation between Seq_elem and Seq_restr
 axiom (forall q: SeqInvoc, s: SetInvoc, n: Invoc :: {Seq_elem(n, Seq_restr(q, s))}
-  Seq_elem(n, Seq_restr(q, s)) <==> Seq_elem(n, q) && Set_elem(n, s));
+  Seq_elem(n, Seq_restr(q, s)) <==> Seq_elem(n, q) && s[n]);
 
 
 // Implicit (strict) order of a sequence
@@ -179,7 +177,7 @@ function Seq_ord(q: SeqInvoc, n1, n2: Invoc) : bool;
 axiom (forall q: SeqInvoc, s: SetInvoc, n: Invoc ::
     {Seq_append(Seq_restr(q, s), n)}
   (forall n1: Invoc :: Seq_elem(n1, Seq_restr(q, s)) ==> Seq_ord(q, n1, n))
-  && Seq_elem(n, q) && !Set_elem(n, s)
+  && Seq_elem(n, q) && !s[n]
   ==> Seq_restr(q, Set_add(s, n)) == Seq_append(Seq_restr(q, s), n));
 
 // Appending extends order
@@ -188,3 +186,4 @@ axiom (forall q: SeqInvoc, n, n1, n2: Invoc :: {Seq_ord(Seq_append(q, n), n1, n2
   (Seq_ord(Seq_append(q, n), n1, n2)
     <==> (Seq_elem(n1, q) && Seq_elem(n2, q) && Seq_ord(q, n1, n2))
       || (Seq_elem(n1, q) && n2 == n)));
+
